$$
\begin{align*}
\text{Taylor Series:} & \quad f(x) = f(a) + f'(a)(x-a) + \frac{f''(a)}{2!}(x-a)^2 + \frac{f'''(a)}{3!}(x-a)^3 + \cdots \\ 

% \sin x &= x - \frac{x^3}{3!} + \frac{x^5}{5!} - \frac{x^7}{7!} + \cdots \\

% \cos x &= 1 - \frac{x^2}{2!} + \frac{x^4}{4!} - \frac{x^6}{6!} + \cdots \\

% \arcsin x &= x + \frac{1}{2} \times \frac{x^3}{3} + \frac{1 \times 3}{2 \times 4} \times \frac{x^5}{5!} + \frac{1 \times 3 \times 5}{2 \times 4 \times 6} \times \frac{x^7}{7!} + \cdots \\

\sin x &= x - \frac{x^3}{3!} + o(x^3) \\
\cos x &= 1 - \frac{x^2}{2!} + \frac{x^4}{4!} + o(x^4) \\

\arcsin x &= x + \frac{x^3}{3!} + o(x^3) \\

\tan x &= x + \frac{x^3}{3} + o(x^3) \\

\arctan x &= x - \frac{1}{3} x^3 + o(x^3) \\

\ln(1+x) &= x - \frac{x^2}{2} + \frac{x^3}{3} + o(x^3) \\

e^x &= 1 + x + \frac{x^2}{2!} + \frac{x^3}{3!} + o(x^3) \\

(1 + x)^a &= 1 + ax + \frac{a(a-1)}{2!}x^2 + o(x^2) \\

\end{align*}
$$